LiveVerif/src/LiveVerif/LiveVerifLib.v
@@ -33,5 +33,6 @@ Require Export coqutil.Datatypes.RecordSetters.
 Require Export LiveVerif.LiveRules.
 Require Export LiveVerif.PackageContext.
 Require Export LiveVerif.LiveProgramLogic.
+Require Export bedrock2.tweak_tacs. Ltac tweak_sidecond_hook ::= try solve [steps].
 Require Export LiveVerif.LiveParsing.
 Require Coq.derive.Derive.
