LiveVerif/src/LiveVerifExamples/sort3_separate_args.v
@@ -49,12 +49,15 @@ step. step. step. step. step. step. step. step. step. step. step. step.
 step.
 (* TODO automate *)
 subst_all_let_bound_vars.
+Import coqutil.Tactics.ident_ops.
+repeat match goal with
+       | H: ?x = _ |- _ => ident_starts_with Def H; subst x
+       end.
 destruct_ifs.
 all: bottom_up_simpl_in_goal.
 all: bottom_up_simpl_in_hyps.
-all: split.
+all: split; [ | lia].
 all: eauto with prove_post.
-all: lia.
 Qed.
 
 End LiveVerif. Comments .**/ //.
