bedrock2/src/bedrock2/find_hyp.v
@@ -28,6 +28,41 @@ Ltac beta1 func arg :=
   | (fun a => ?f) => constr:(subst! arg for a in f)
   end.
 
+Ltac find_hyp_by_pat_TOO_SLOW_1 patfun :=
+  let does_match t :=
+    let _ := constr:(fun fff: False => ltac:(
+        let b := beta1 patfun fff in
+        let _ := matches t b in
+        exact fff)) in
+    idtac in
+  match goal with
+  | H1: context[?x1] |- _ =>
+      does_match x1;
+      tryif match goal with
+            | H2: context[?x2] |- _ =>
+                tryif constr_eq H1 H2 then fail
+                else (does_match x2; fail 3 "non-unique pattern matches both" H1 "and" H2)
+            end
+      then fail 1000 "whoops, should already have failed earlier"
+      else exact H1
+  end.
+
+Ltac multi_find_hyp_by_pat patfun :=
+  multimatch goal with
+  | H: context[?x] |- _ =>
+      let _ := constr:(fun fff: False => ltac:(
+        let b := beta1 patfun fff in
+        let _ := matches x b in
+        exact fff))
+      in exact H
+  end.
+
+(* Note: imprecise error message "This tactic has more than one success", would be
+   better to report "non-unique pattern matches both H1 and H2" *)
+Ltac find_hyp_by_pat_TOO_SLOW_2 patfun := exactly_once (idtac; multi_find_hyp_by_pat patfun).
+
+(* TODO can we raise an error if more than one hypothesis match, but without too
+   much slowdown? *)
 Ltac find_hyp_by_pat patfun :=
   match goal with
   | H: context[?x] |- _ =>
@@ -41,17 +76,20 @@ Ltac find_hyp_by_pat patfun :=
 Notation "??" := ltac:(match goal with ff: False |- _ => case ff end) (only parsing).
 
 Declare Custom Entry pat.
-Notation "b" := (fun ff: False => b) (in custom pat at level 0, b constr at level 200).
+Notation "b" := (fun ff: False => b) (in custom pat at level 0, b constr at level 0).
 
-Notation "'find!' p" := ltac:(find_hyp_by_pat p)
-  (at level 10, p custom pat at level 0, only parsing).
+Notation "# p" := ltac:(find_hyp_by_pat p)
+  (at level 6, p custom pat at level 0, only parsing).
 
 Goal forall a b: nat, a = 5 -> a < b -> a < 3 /\ 1 <= a -> a < 4 /\ b < 4 -> False.
   intros.
-  pose proof (find! (?? < b)).
-  eassert (_) by exact (find! (1 <= ??)).
-  pose proof (find! (a < ?? /\ ?? < 4)).
-  let HH := constr:(find! (a < b)) in rewrite (find! (a = ??)) in HH.
+  pose proof #(?? < b) as AB.
+  pose proof #(?? < b). (* this should fail with non-uniqueness error *)
+  clear AB.
+  eassert (_) as P by exact #(1 <= ??).
+  clear P.
+  pose proof #(a < ?? /\ ?? < 4).
+  let HH := constr:(#(a < b)) in rewrite #(a = ??) in HH.
   let rew := (fun Heq Hwhere => rewrite Heq in Hwhere) in
-  rew (find! (a = ??)) (find! (1 <= ??)).
+  rew #(a = ??) #(1 <= ??).
 Abort.
